clightplus/compiler_proof/ClightPlus2ClightSepComp.v
@@ -61,15 +61,11 @@ Section PROOFSINGLE.
 
   Ltac wrap_up := try pfold; econs 7; et; right.
 
-  Definition compile_val mdl := @ModL.compile _ EMSConfigC mdl. 
+  Definition compile_val mdl := @ModL.compile _ EMSConfigC mdl.
 
   Definition clightp_sem sk_mem md := compile_val (ModL.add (Mod.lift (Mem sk_mem)) (Mod.lift md)).
 
   Definition clightp_initial_state sk_mem md := (clightp_sem sk_mem md).(STS.initial_state).
-
-  Definition mem_keywords := List.map ident_of_string ["malloc"; "free"; "capture"].
-
-  Definition sk_mem (clight_prog: Clight.program) := List.map (map_fst string_of_ident) (List.filter (fun x => in_dec Pos.eq_dec (fst x) mem_keywords) (prog_defs clight_prog)).
 
   Local Opaque ident_of_string.
   Arguments Es_to_eventE /.
@@ -77,63 +73,36 @@ Section PROOFSINGLE.
   Arguments sloop_iter_body_two /.
   Arguments ktree_of_cont_itree /.
 
-  Lemma asdf' clight_prog mn md str gd:
-    compile clight_prog mn = Some md ->
-    In (str, gd) (Sk.canon (Sk.add (sk_mem clight_prog) (Mod.sk md))) ->
-    In (ident_of_string str, gd) (prog_defs clight_prog).
-  Proof.
-    i. unfold compile in H. unfold get_sk in H. des_ifs. ss. bsimpl. des.
-    let x := type of Sk.le_canon_rev in
-    let y := eval red in x in
-    eapply (Sk.le_canon_rev: x) in H0.
-    ss. apply in_map with (f:=(map_fst ident_of_string)) in H0. ss.
-    unfold Sk.add in H0. ss. rewrite map_app in H0. rewrite List.in_app_iff in H0.
-    unfold sk_mem in H0. clear - H0 Heq1. revert_until clight_prog.
-    generalize (prog_defs clight_prog). clear. induction l; i; ss; try tauto.
-    des_ifs.
-    - ss. bsimpl. des.
-      + left. destruct a. ss. clarify. rewrite string_of_ident_of_string in H1. f_equal; et.
-      + right. eapply IHl; et.
-      + left. destruct a. ss. clarify. rewrite string_of_ident_of_string in H1. f_equal; et.
-      + right. eapply IHl; et.
-    - ss. bsimpl. des; clarify.
-      + left. destruct a. ss. clarify. rewrite string_of_ident_of_string in H1. f_equal; et.
-      + left. destruct a. ss. clarify. rewrite string_of_ident_of_string in H1. f_equal; et.
-      + right. eapply IHl; et.
-      + right. eapply IHl; et.
-      + left. destruct a. ss. clarify. rewrite string_of_ident_of_string in H1. f_equal; et.
-      + left. destruct a. ss. clarify. rewrite string_of_ident_of_string in H1. f_equal; et.
-      + right. eapply IHl; et.
-      + right. eapply IHl; et.
-    - ss. bsimpl. des; clarify.
-      + left. destruct a. ss. clarify. rewrite string_of_ident_of_string in H1. f_equal; et.
-      + right. eapply IHl; et.
-      + right. eapply IHl; et.
-    - ss. bsimpl. des; clarify.
-      + left. destruct a. ss. clarify. rewrite string_of_ident_of_string in H1. f_equal; et.
-      + left. destruct a. ss. clarify. rewrite string_of_ident_of_string in H1. f_equal; et.
-      + right. eapply IHl; et.
-      + right. eapply IHl; et.
-      + right. eapply IHl; et.
-      + right. eapply IHl; et.
-    - ss. bsimpl. des; clarify.
-      + right. eapply IHl; et.
-      + left. destruct a. ss. clarify. unfold chk_ident in Heq1. destruct Pos.eq_dec; clarify. rewrite <- e in H1. f_equal; et.
-      + right. eapply IHl; et.
-    - ss. bsimpl. des; clarify.
-      + right. eapply IHl; et.
-      + right. eapply IHl; et.
-  Qed.
+  (* mem initialization condition : every Gvar has aligned and every Gvar address is in genv *)
+  (* src align <-> tgt align is valid, Gvar is remain in both *)
+  (* second condition makes src valid addr -> tgt valid addr but not inverse *)
+  (* so, src init succ -> tgt init succ *)
+  (* compiler should check whether src init is a success *)
+  (* suggestion 1: compiler initialize its memory *)
 
-  Lemma asdf clight_prog mn md idx str:
+  (* if address points to external name *)
+  (* restrict thm to src initialization success (total program) *)
+  (* or ub when initialization fails *)
+
+  Lemma compile_init_mem_success clight_prog mn md tm:
     compile clight_prog mn = Some md ->
-    SkEnv.blk2id (load_skenv (Sk.canon (Sk.add (sk_mem clight_prog) (Mod.sk md)))) idx = Some str ->
-    exists tb, Genv.find_symbol (Genv.globalenv clight_prog) (ident_of_string str) = Some tb.
+    Genv.init_mem clight_prog = Some tm ->
+    exists m, load_mem (Sk.canon (Sk.add (sk_mem clight_prog) (Mod.sk md))) = Some m /\ match_mem (Sk.canon (Sk.add (sk_mem clight_prog) (Mod.sk md))) (globalenv clight_prog) m tm.
+
+  Lemma init_memory clight_prog mn md tm:
+    compile clight_prog mn = Some md ->
+    Genv.init_mem clight_prog = Some tm ->
+    exists m, load_mem (Sk.canon (Sk.add (sk_mem clight_prog) (Mod.sk md))) = Some m /\ match_mem (Sk.canon (Sk.add (sk_mem clight_prog) (Mod.sk md))) (globalenv clight_prog) m tm.
   Proof.
-    i. hexploit in_env_in_sk; et. i. des. clear H0.
-    apply Genv.find_symbol_exists with (g:=def).
-    eapply asdf'; et.
-  Qed.
+    i. assert (forall str gd, In (str, gd) (Sk.canon (Sk.add (sk_mem clight_prog) (Mod.sk md))) -> In (ident_of_string str, gd) (prog_defs clight_prog)) by now intros str gd; eapply asdf'; et.
+    set (Sk.canon _) as sk_init in *. clearbody sk_init.
+    unfold load_mem, Genv.init_mem in *.
+    assert
+    unfold compile, get_sk, sk_mem. i.
+    des_ifs. ss. 
+
+    clearbody sk_init.
+
 
   (* This single thm will be used in final thm. *)
   Theorem single_compile_behavior_improves
@@ -167,34 +136,11 @@ Section PROOFSINGLE.
     eapply sim_bot_flag_up with (b0 := true) (b1 := false).
 
     set (sort _) as sk_init in *.
+    hexploit compile_match_genv; et. i.
     eapply step_function_entry with (modl:=md) (tm:=m0) (ge:=globalenv clight_prog) (sk:=sk_init); et.
-    { unfold sk_init. econs.
-      - change sort with (@Sk.canon _). apply Sk.wf_canon. unfold ModL.wf in w. ss. des. et.
-      - i. unfold ModL.wf in w. ss. des. apply Sk.wf_canon in SK.
-        hexploit load_skenv_wf; et. i. unfold SkEnv.wf in H2. red in H2. rewrite H2 in H1.
-        hexploit asdf; et. i. clear H2.
-        des. unfold map_blk. destruct le_dec; cycle 1.
-        { replace (Init.Nat.pred _) with idx by nia. ss. rewrite H1.
-          des_ifs. unfold fundef in *. clarify. }
-        exfalso. assert (List.length (sort (Sk.add (sk_mem clight_prog) (Mod.sk md))) <= idx) by nia.
-        Local Transparent load_skenv. ss. uo. des_ifs.
-        apply nth_error_None in H2. clarify.
-      - i. fold sk_init in H1.
-        assert (SkEnv.blk2id (load_skenv sk_init) n = Some s) by now ss; uo; des_ifs.
-        hexploit asdf; et. i. des.
-        assert (Genv.find_symbol (Genv.globalenv clight_prog) (ident_of_string s) = Some (map_blk sk_init (Genv.globalenv clight_prog) (Pos.of_succ_nat n))).
-        { unfold map_blk. destruct le_dec; cycle 1.
-          { replace (Init.Nat.pred _) with n by nia. rewrite H2.
-            des_ifs. unfold fundef in *. clarify. }
-          exfalso. assert (List.length sk_init <= n) by nia. ss. uo. des_ifs.
-          apply nth_error_None in H4. clarify. }
-        clear H3.
-        assert (Maps.PTree.get (ident_of_string s) (prog_defmap clight_prog) = Some gd).
-        { unfold prog_defmap. ss. apply Maps.PTree_Properties.of_list_norepet; et. 
-          { unfold compile, get_sk in COMP. des_ifs. destruct list_norepet_dec; clarify. }
-          apply nth_error_in in H1. unfold sk_init in H1. eapply asdf'; et. }
-        rewrite Genv.find_def_symbol in H3. des. clarify. }
-    { admit "". }
+    { unfold get_ce. ss. econs. split; i.
+      - apply alist_find_some_iff; et. rewrite CoqlibC.NoDup_norepet. apply Maps.PTree.elements_keys_norepet.
+      - eapply alist_find_some; et. }
     { admit "". }
     i. pfold. econs 4. { i. inv H5. et. } { eexists. econs. et. }
     i. inv STEP. econs 8; et. left. 
